Normalize TypeLanguage syntax infrastructure

ContextTypeLanguage/theories/TypeOpen.v
@@ -1,13 +1,137 @@
 (** * ContextTypeLanguage.TypeOpen
 
-    Multi-opening for context types and type qualifiers.
+    Single and finite-map opening for context types and type qualifiers.
 
-    This file is syntax-only: it contains the finite-map opening operations
-    for [context_ty] and [type_qualifier], plus their structural laws.  The
-    lvar-keyed type environment projection machinery stays in [Env.v]. *)
+    This file is syntax-only: it contains the generic finite-map opening
+    infrastructure, the concrete multi-opening operations for [context_ty] and
+    [type_qualifier], plus their structural laws.  The lvar-keyed type
+    environment projection machinery stays in [ContextStore]/[LtyEnv]. *)
 
-From ContextTypeLanguage Require Export MultiOpen.
+From Stdlib Require Import Classes.RelationClasses Classes.Morphisms.
+From LocallyNameless Require Import Classes.
+From ContextTypeLanguage Require Export Syntax.
 From ContextBase Require Import BaseTactics.
+
+(** * Generic finite-map opening infrastructure. *)
+
+Class MOpen Env A B := mopen : Env -> A -> B.
+Arguments mopen {_ _ _ _} _ _.
+
+Notation "η ⊙ x" := (mopen η x)
+  (at level 30, right associativity, format "η  ⊙  x").
+
+Class OpenCommute (A : Type) (openA : nat -> atom -> A -> A)
+    (R : relation A) := {
+  open_commute :
+    forall i j x y (a : A),
+      i <> j ->
+      x <> y ->
+      R (openA i x (openA j y a)) (openA j y (openA i x a));
+}.
+
+Class OpenProper (A : Type) (openA : nat -> atom -> A -> A)
+    (R : relation A) := {
+  open_proper :
+    forall i x, Proper (R ==> R) (openA i x);
+}.
+
+#[global] Instance open_proper_cty_vars_equiv :
+  OpenProper context_ty cty_open cty_vars_equiv.
+Proof.
+  constructor. intros i x τ1 τ2 Hτ.
+  apply cty_vars_equiv_open. exact Hτ.
+Qed.
+
+#[global] Instance open_commute_cty_vars_equiv :
+  OpenCommute context_ty cty_open cty_vars_equiv.
+Proof.
+  constructor. intros i j x y τ Hij Hxy.
+  rewrite cty_open_commute_fvar by assumption. reflexivity.
+Qed.
+
+#[global] Instance open_commute_cty_eq :
+  OpenCommute context_ty cty_open eq.
+Proof.
+  constructor. intros i j x y τ Hij Hxy.
+  apply cty_open_commute_fvar; assumption.
+Qed.
+
+#[global] Instance open_commute_lvars :
+  OpenCommute lvset lvars_open eq.
+Proof.
+  constructor. intros i j x y D Hij Hxy.
+  rewrite set_swap_conjugate.
+  replace (swap (LVBound i) (LVFree x) (LVBound j)) with (LVBound j).
+  2:{ unfold swap. repeat destruct decide; congruence. }
+  replace (swap (LVBound i) (LVFree x) (LVFree y)) with (LVFree y).
+  2:{ unfold swap. repeat destruct decide; congruence. }
+  reflexivity.
+Qed.
+
+#[global] Instance open_commute_qual_eq :
+  OpenCommute type_qualifier qual_open_atom eq.
+Proof.
+  constructor. intros i j x y q Hij Hxy.
+  apply qual_open_commute_fvar; assumption.
+Qed.
+
+Class MOpenInsertLaws A B `{Open atom A}
+    `{MOpen (gmap nat atom) A B} := {
+  mopen_insert_norm :
+    forall k x η (a : A),
+      η !! k = None ->
+      open_env_avoids_atom x η ->
+      mopen η ({k ~> x} a) = mopen (<[k := x]> η) a;
+}.
+
+Lemma open_map_fold_insert_fresh_eq
+    {A : Type} (openA : nat -> atom -> A -> A)
+    `{!OpenCommute A openA eq}
+    (η : gmap nat atom) k x (a : A) :
+  η !! k = None ->
+  open_env_avoids_atom x η ->
+  open_env_values_inj η ->
+  map_fold openA a (<[k := x]> η) =
+  openA k x (map_fold openA a η).
+Proof.
+  intros Hfresh Havoid Hinj.
+  apply (map_fold_insert_L (M:=gmap nat) (A:=atom) (B:=A)
+    openA a k x η).
+  - intros i j xi xj acc Hij Hi Hj.
+    apply open_commute; [exact Hij|].
+    intros Heq. subst xj.
+    pose proof (open_env_values_inj_insert k x η Hfresh Havoid Hinj)
+      as Hinj'.
+    apply Hij. eapply Hinj'; eassumption.
+  - exact Hfresh.
+Qed.
+
+Lemma open_map_fold_insert_fresh_rel
+    {A : Type} (R : relation A) `{!PreOrder R}
+    (openA : nat -> atom -> A -> A)
+    `{HproperInst : !OpenProper A openA R}
+    `{HcommuteInst : !OpenCommute A openA R}
+    (η : gmap nat atom) k x (a : A) :
+  η !! k = None ->
+  open_env_avoids_atom x η ->
+  open_env_values_inj η ->
+  R (map_fold openA a (<[k := x]> η))
+    (openA k x (map_fold openA a η)).
+Proof.
+  intros Hfresh Havoid Hinj.
+  destruct HproperInst as [Hproper].
+  destruct HcommuteInst as [Hcommute].
+  eapply (map_fold_insert (M := gmap nat) (A := atom) (B := A)
+    R openA a k x η).
+  - intros i y. apply Hproper.
+  - intros i j xi xj acc Hij Hi Hj.
+    apply Hcommute; [exact Hij|].
+    intros Heq. subst xj.
+    pose proof (open_env_values_inj_insert k x η Hfresh Havoid Hinj)
+      as Hinj'.
+    apply Hij. eapply Hinj'; eassumption.
+  - exact Hfresh.
+Qed.
 
 Definition open_cty_env (η : gmap nat atom) (τ : context_ty) : context_ty :=
   map_fold (fun k x acc => cty_open k x acc) τ η.
@@ -684,3 +808,51 @@ Proof.
     rewrite open_cty_env_insert_fresh by assumption.
     reflexivity.
 Qed.
+
+(** * ContextTypeLanguage.TypeOpen
+
+    Syntax-shape normalization tactics for finite-map opening. *)
+
+Ltac qual_open_env_syntax_norm :=
+  rewrite ?qual_open_env_empty;
+  try rewrite ?qual_open_env_insert_fresh by eauto;
+  try rewrite ?qual_open_env_vars by eauto.
+
+Ltac qual_open_env_syntax_norm_in H :=
+  rewrite ?qual_open_env_empty in H;
+  try rewrite ?qual_open_env_insert_fresh in H by eauto;
+  try rewrite ?qual_open_env_vars in H by eauto.
+
+Ltac cty_open_env_syntax_norm :=
+  rewrite ?open_cty_env_empty;
+  rewrite ?open_cty_env_preserves_erasure;
+  rewrite ?open_cty_env_inter, ?open_cty_env_union, ?open_cty_env_sum;
+  try rewrite ?open_cty_env_arrow by eauto;
+  try rewrite ?open_cty_env_wand by eauto;
+  try rewrite ?open_cty_env_over by eauto;
+  try rewrite ?open_cty_env_under by eauto;
+  try rewrite ?context_ty_lvars_open_cty_env by eauto;
+  try rewrite ?open_cty_env_lift_shift0_exact by eauto.
+
+Ltac cty_open_env_syntax_norm_in H :=
+  rewrite ?open_cty_env_empty in H;
+  rewrite ?open_cty_env_preserves_erasure in H;
+  rewrite ?open_cty_env_inter in H;
+  rewrite ?open_cty_env_union in H;
+  rewrite ?open_cty_env_sum in H;
+  try rewrite ?open_cty_env_arrow in H by eauto;
+  try rewrite ?open_cty_env_wand in H by eauto;
+  try rewrite ?open_cty_env_over in H by eauto;
+  try rewrite ?open_cty_env_under in H by eauto;
+  try rewrite ?context_ty_lvars_open_cty_env in H by eauto;
+  try rewrite ?open_cty_env_lift_shift0_exact in H by eauto.
+
+Ltac type_open_env_syntax_norm :=
+  qual_open_env_syntax_norm;
+  cty_open_env_syntax_norm;
+  type_syntax_norm.
+
+Ltac type_open_env_syntax_norm_in H :=
+  qual_open_env_syntax_norm_in H;
+  cty_open_env_syntax_norm_in H;
+  type_syntax_norm_in H.
